networkInvariantPrototypes/paxos/monotonic/messageInvariants.dfy
@@ -22,6 +22,36 @@ predicate ValidMessageSrc(c: Constants, v: Variables)
     case Learn(lnr, _, _) => c.ValidLearnerIdx(lnr)
 }
 
+// Message bundle
+predicate MessageInv(c: Constants, v: Variables) 
+{
+  && v.WF(c)
+  && ValidMessageSrc(c, v)
+  && LeaderValidHighestHeard(c, v)
+  && LeaderValidReceivedPromises(c, v)
+  && AcceptorValidPromised(c, v)
+  && AcceptorValidAcceptedVB(c, v)
+  && LearnerValidReceivedAccepts(c, v)
+}
+
+lemma InitImpliesMessageInv(c: Constants, v: Variables)
+  requires Init(c, v)
+  ensures MessageInv(c, v)
+{
+}
+
+lemma MessageInvInductive(c: Constants, v: Variables, v': Variables)
+  requires MessageInv(c, v)
+  requires Next(c, v, v')
+  ensures MessageInv(c, v')
+{
+  InvNextAcceptorValidPromised(c, v, v');
+}
+
+/***************************************************************************************
+*                                     Leader Host                                      *
+***************************************************************************************/
+
 // certified self-inductive
 // Leader updates its highestHeard and value based on a Promise message carrying that
 // ballot and value
@@ -48,17 +78,21 @@ predicate LeaderValidReceivedPromises(c: Constants, v: Variables)
     )
 } 
 
+/***************************************************************************************
+*                                     Acceptor Host                                    *
+***************************************************************************************/
+
 // certified self-inductive
 // Acceptor updates its promised ballot based on a Prepare/Propose message carrying 
-// that ballot
+// that ballot. Derived from only NextReceiveStep
 predicate AcceptorValidPromised(c: Constants, v: Variables)
   requires v.WF(c)
 {
-  forall idx, b | c.ValidAcceptorIdx(idx) && v.acceptors[idx].promised == Some(b)
-  :: (exists m: Message ::
-        && (IsPromiseMessage(v, m) || IsProposeMessage(v, m))
-        && m.bal == b
-    )
+  forall idx, i | 
+    && c.ValidAcceptorIdx(idx) 
+    && 0 <= i < |v.acceptors[idx].promised|
+  :: 
+    ExistsIsPrepareOrPropose(c, v, idx, i)
 }
 
 // certified self-inductive
@@ -67,13 +101,19 @@ predicate AcceptorValidPromised(c: Constants, v: Variables)
 predicate AcceptorValidAcceptedVB(c: Constants, v: Variables)
   requires v.WF(c)
 {
-  forall idx, val, bal | 
+  forall idx, i | 
     && c.ValidAcceptorIdx(idx) 
-    && v.acceptors[idx].acceptedVB == Some(VB(val, bal))
+    && 0 <= i < |v.acceptors[idx].acceptedVB|
   :: 
-    && Propose(bal, val) in v.network.sentMsgs
-    && Accept(VB(val, bal), c.acceptorConstants[idx].id) in v.network.sentMsgs
+    && var vb := v.acceptors[idx].acceptedVB[i];
+    && Propose(vb.b, vb.v) in v.network.sentMsgs
+    && Accept(vb, c.acceptorConstants[idx].id) in v.network.sentMsgs
 }
+
+
+/***************************************************************************************
+*                                     Learner Host                                     *
+***************************************************************************************/
 
 
 
@@ -91,29 +131,54 @@ predicate LearnerValidReceivedAccepts(c: Constants, v: Variables)
     Accept(vb, acc) in v.network.sentMsgs
 }
 
-// Message bundle
-predicate MessageInv(c: Constants, v: Variables) 
-{
-  && v.WF(c)
-  && ValidMessageSrc(c, v)
-  && LeaderValidHighestHeard(c, v)
-  && LeaderValidReceivedPromises(c, v)
-  && AcceptorValidPromised(c, v)
-  && AcceptorValidAcceptedVB(c, v)
-  && LearnerValidReceivedAccepts(c, v)
-}
 
-lemma InitImpliesMessageInv(c: Constants, v: Variables)
-  requires Init(c, v)
-  ensures MessageInv(c, v)
-{
-}
+/***************************************************************************************
+*                               Proofs (how unfortunate)                               *
+***************************************************************************************/
 
-lemma MessageInvInductive(c: Constants, v: Variables, v': Variables)
-  requires MessageInv(c, v)
+// Tony: This message invariant requires proof. What do I make of this?
+// Also the copy-pasta for the unchanged cases are is gross
+lemma InvNextAcceptorValidPromised(c: Constants, v: Variables, v': Variables)
+  requires v.WF(c)
+  requires v'.WF(c)
+  requires AcceptorValidPromised(c, v)
   requires Next(c, v, v')
-  ensures MessageInv(c, v')
-{}
+  ensures AcceptorValidPromised(c, v')
+{
+  forall idx, i | 
+    && c.ValidAcceptorIdx(idx) 
+    && 0 <= i < |v'.acceptors[idx].promised|
+  ensures
+    ExistsIsPrepareOrPropose(c, v', idx, i)
+  {
+    var dsStep :| NextStep(c, v, v', dsStep);
+    var actor, msgOps := dsStep.actor, dsStep.msgOps;
+    if dsStep.AcceptorStep? && idx == actor && i == |v'.acceptors[idx].promised| - 1 {
+      var ac, a, a' := c.acceptorConstants[idx], v.acceptors[idx], v'.acceptors[idx];
+      var step :| AcceptorHost.NextStep(ac, a, a', step, msgOps);
+      if step.ReceiveStep? {
+        var m := msgOps.recv.value;
+        if m.Prepare? && (a.PromisedNone() || a.GetPromised() < m.bal) {
+          assert IsPrepareOrPropose(v', m, a'.promised[i]);  // trigger
+        } else if m.Propose? && (a.PromisedNone() || a.GetPromised() <= m.bal) {
+          assert IsPrepareOrPropose(v', m, a'.promised[i]);  // trigger
+        } else {
+          assert ExistsIsPrepareOrPropose(c, v, idx, i);                    // trigger
+          var m :| IsPrepareOrPropose(v, m, v.acceptors[idx].promised[i]);  // witness
+          assert IsPrepareOrPropose(v', m, v'.acceptors[idx].promised[i]);  // trigger
+        }
+      } else {
+        assert ExistsIsPrepareOrPropose(c, v, idx, i);                    // trigger
+        var m :| IsPrepareOrPropose(v, m, v.acceptors[idx].promised[i]);  // witness
+        assert IsPrepareOrPropose(v', m, v'.acceptors[idx].promised[i]);  // trigger
+      }
+    } else {
+      assert ExistsIsPrepareOrPropose(c, v, idx, i);                    // trigger
+      var m :| IsPrepareOrPropose(v, m, v.acceptors[idx].promised[i]);  // witness
+      assert IsPrepareOrPropose(v', m, v'.acceptors[idx].promised[i]);  // trigger
+    }
+  }
+}  
 
 /***************************************************************************************
 *                                        Utils                                         *
@@ -143,5 +208,22 @@ predicate IsLearnMessage(v: Variables, m: Message) {
   && m.Learn?
   && m in v.network.sentMsgs
 } 
+
+predicate IsPrepareOrPropose(v: Variables, m: Message, bal: LeaderId) {
+  && m in v.network.sentMsgs
+  && (m.Prepare? || m.Propose?)
+  && m.bal == bal
+}
+
+// Tony: Dafny is somehow unable to prove AcceptorValidPromised(c, v') if the exists is
+// not wrapped in such a predicate
+predicate ExistsIsPrepareOrPropose(c: Constants, v: Variables, idx: nat, i: int) 
+  requires v.WF(c)
+  requires c.ValidAcceptorIdx(idx) 
+  requires 0 <= i < |v.acceptors[idx].promised|
+{
+  exists m :: IsPrepareOrPropose(v, m, v.acceptors[idx].promised[i])
+}
+
 }  // end module PaxosProof
 
